Updated setup with new changes

noc/setup.v
@@ -6,7 +6,8 @@ Require Import noc.helpers.
 Require Import Coq.Vectors.Fin.
 
 From Equations Require Import Equations.
-(* Set Equations Transparent. *)
+Set Equations Transparent.
+
 
 Module Setup.
 
@@ -62,13 +63,14 @@ End Setup.
 Module Instances.
 
   Import Setup Helpers.
-
   Derive Signature for reg_t.
   Derive NoConfusion for reg_t.
-
+  
   Equations fin_idx {n} (r: (reg_t (S n))) : nat :=
-    fin_idx (router _ n' state)      := 2 * proj1_sig (Fin.to_nat n');
-    fin_idx (router _ n' downstream) := 2 * proj1_sig (Fin.to_nat n') + 1.
+  fin_idx (router _ (@F1 n')   state) := 2 * n';
+  fin_idx (router _ (@FS n' _) state) := 2 * n';
+  fin_idx (router _ (@F1 n')   downstream) := 2 * n' + 1;
+  fin_idx (router _ (@FS n' _) downstream) := 2 * n' + 1.
 
   (* TODO move rename to [widen_le_t] *)
   Equations widen_fin_left {m} (H: m <<= S (S m)) : S m <<= S (S m) :=
@@ -84,81 +86,59 @@ Module Instances.
      le_S _ _ (widen_le_t_S H').
 
   Equations fin_elems' n m (H: n <<= m) : list (reg_t (S m)) :=
-    fin_elems' 0      0     _  :=
-      [router 0 F1 state; router 0 F1 downstream];
-
+    fin_elems' 0      0     _               := cons (router 0 F1 state) (cons (router 0 F1 downstream) nil);
     fin_elems' 0     (S 0) (le_S 0 ?(0) H') :=
       let f1 := FS (@F1 0) in
-      [router (S 0) f1 state; router (S 0) f1 downstream];
+      cons (router (S 0) f1 state) (cons (router (S 0) f1 downstream) nil);
 
-    fin_elems' 0     (S (S m')) H' :=
-      let f1 := FS (widen_fin (widen_fin_left0 H') (@F1 0)) in
-      [router (S (S m')) f1 state; router (S (S m')) f1 downstream];
+  fin_elems' 0     (S (S m')) H' :=
+    let f1 := FS (widen_fin (widen_fin_left0 H') (@F1 0)) in
+    cons (router (S (S m')) f1 state) (cons (router (S (S m')) f1 downstream) nil);
 
-    fin_elems' (S n') (S m') H' with fin_elems' n' (S m') (le_t_inj H') :=
-      | tl := let f1 := widen_fin (widen_le_t_S H') (@F1 (S n')) in
-              cons (router (S m') f1 state)
-                (cons (router (S m') f1 downstream) tl).
-
+  fin_elems' (S n') (S m') H' with fin_elems' n' (S m') (le_t_inj H') :=
+    | tl := let f1 := widen_fin (widen_le_t_S H') (@F1 (S n')) in
+            cons (router (S m') f1 state)
+              (cons (router (S m') f1 downstream) tl).   
 
   Definition fin_elems {n} : list (reg_t (S n)) :=
     fin_elems' n n (le_n n).
 
-  Lemma regt_error :
-    forall n, forall a: (reg_t (S n)),
-      List.nth_error fin_elems (fin_idx a) = Some a.
+  Equations lift {m} (l: list (reg_t m)) : list (reg_t (S m)) :=
+    lift nil := nil;
+    lift (cons (router m f s) tl) with lift tl => {
+        | tl' := cons (router (S m) (FS f) s) tl'
+      }.
+  
+  Equations fin_elems'' m : list (reg_t (S m)) :=
+    fin_elems'' 0      := cons (router 0 F1 state) (cons (router 0 F1 downstream ) nil);
+    fin_elems'' (S m') with fin_elems'' m' => {
+      | tl := cons (router (S m') (@F1 (S m')) state)
+                (cons (router (S m') (@F1 (S m')) downstream)
+                   (lift tl))
+        }.
+  
+  Lemma help: forall n m',
+    List.nth_error (fin_elems'' m') n = Some (router m' F1 state) ->
+    List.nth_error (lift (fin_elems'' m')) n = Some (router (S m') F1 state).
+  Admitted.
+
+    Lemma regt_error :
+    forall n, forall (r: (reg_t (S n))),
+      List.nth_error (fin_elems'' n) (fin_idx r) = Some r.
   Proof.
-    intros n r.
-    unfold fin_elems.
-    funelim (fin_elems' n n (le_n n)).
-    - simp fin_elems'.
-      depelim r.
-      depelim t; try inversion t.
-      funelim (fin_idx (router 0 F1 r));
-      rewrite <- Heqcall;
-      depelim n'; simpl; inversion H; rewrite H1; reflexivity.
-    - simp fin_elems'.
-      cbv zeta.
-      (* rewrite <- H0; rewrite <- H1; clear H0 H1. *)
-      (* simp widen_le_t_S. *)
-      depelim r.
-      depelim t.
-      + funelim (fin_idx (router (S n') F1 r));
-        inversion H; clear H;
-        simp fin_idx; simpl; reflexivity.
-      + specialize (Hind (S n') (router (S n') (FS t) r)).
-        simp le_t_inj in Hind.
-        revert Hind.
-        funelim (fin_idx (router (S n') (FS t) r)).
-        * inversion H; clear H;
-          simp fin_idx; simpl.
+  intros n r.
+  funelim (fin_elems'' n).
+  - funelim (fin_idx r). simp fin_idx; simpl; try (reflexivity || depelim f).
+  - funelim (fin_idx r); simp fin_idx; simpl; rewrite <- plus_n_O.
+    + Search (_ + S _).
+      rewrite <- plus_n_Sm.
+      simpl.
+      specialize (Hind (mk m' F1 A)).
+      simp fin_idx in Hind.
+      simpl in Hind.
+      rewrite <- plus_n_O in Hind.
 
-          rewrite Nat.add_0_r.
-          assert (n'_eq_fs_t := inj_right_pair H1).
-          (* rewrite <- n'_eq_fs_t. *)
-          simpl.
-          destruct (to_nat t).
-          simpl proj1_sig.
-
-          simpl.
-          rewrite <- plus_n_Sm.
-          simpl.
-          simp fin_elems'.
-          cbv zeta.
-          simpl.
-          simp widen_le_t_S.
-          intro Hind.
-          apply Hind.
-
-          specialize (H eq_refl).
-          apply H.
-          specialize (H (S n'0) (router (S n'0) n' state)).
-          simp le_t_inj in H.
-
-          clear H2.
-          apply H.
-          rewrite n'_eq_fs_t in H.
-          rewrite <- Heqcall in H.
+  
 
   Instance Fin_regt : forall n, FiniteType (reg_t (S n)) :=
   {
